SecureMessaging.lean
@@ -50,6 +50,7 @@ import SecureMessaging.SCKA.MLKEMBraid.Basic
 import SecureMessaging.SCKA.MLKEMBraid.Construction
 import SecureMessaging.SCKA.SPQR.Chunked
 import SecureMessaging.SCKA.SPQR.Construction
+import SecureMessaging.SCKA.SPQR.Correspondence
 import SecureMessaging.SCKA.SPQR.Instances
 import SecureMessaging.SCKA.SPQR.Unchunked
 import SecureMessaging.SCKA.OppUniKEM.Construction
